



$$e_1 = R - y$$

$$e_2 = e_1 - H_1 V, \quad e_2 = R - y - H_1 V$$

$$u = x - H_2 y = R - y - H_1 G_1 (G_1 e_2 - H_2 y)$$

$$x = G_1 e_2 \quad e_2 (1 + H_1 G_1 G_2) = R + y [H_1 G_2 H_2 - 1]$$

$$V = G_2 u \quad e_2 = \frac{R + y [H_1 H_2 G_2 - 1]}{1 + H_1 G_1 G_2}$$

$$w = G_3 V$$

$$y = w + G_4 e_2 + N$$

$$V = G_2 (G_1 e_2 - H_2 y)$$

$$w = G_3 G_2 (G_1 e_2 - H_2 y)$$

$$y = G_3 G_2 (G_1 e_2 - H_2 y) + G_4 e_2 + N$$

$$y (1 + H_2 G_2 G_3) = G_3 G_2 G_3 e_2 + G_4 e_2 + N$$

$$y [1 + H_2 G_2 G_3] = \frac{G_4 + G_1 G_2 G_3}{1 + H_1 G_1 G_2} [R + y [H_1 H_2 G_2 - 1]] + N$$

$$y [1 + H_1 G_1 G_2] [1 + H_2 G_2 G_3] + [1 - H_1 H_2 G_2] [G_1 G_2 G_3 + G_4] = R [G_1 G_2 G_3 + G_4] + N [1 + H_1 G_1 G_2]$$